Allow Dirents to be more than one block
We now enforce the restriction in MemDirents and in dir_fs, in
preparation for large directories. Dirents has a bunch of useful theory
for pure DirEnt sequences that's well-organized without factoring out
properties of seq<DirEnt> (actually there's a bunch of theory in the
file for those, too, but right now they just serve as lemmas).

src/Dafny/examples/fs/dirent.dfy
@@ -344,7 +344,7 @@ module DirEntries
     predicate Valid()
     {
       // 128*32 == 4096 so these will fit in a block
-      && |s| == dir_sz
+      && |s| <= dir_sz
       && dirents_unique(s)
     }
 
@@ -362,7 +362,7 @@ module DirEntries
 
     lemma enc_len()
       requires Valid()
-      ensures |enc()| == 4096
+      ensures |enc()| == dirent_sz*|s|
     {
       C.concat_homogeneous_len(C.seq_fmap(encOne, this.s), dirent_sz);
     }
